src/RqRsInv.v
@@ -1,7 +1,7 @@
 Require Import Peano_dec List ListSupport.
 Require Import Common FMap.
 Require Import Syntax Semantics StepM Invariant Serial.
-Require Import Reduction Commutable QuasiSeq Topology.
+Require Import Reduction Commutativity QuasiSeq Topology.
 Require Import RqRsTopo.
 
 Set Implicit Arguments.
@@ -43,9 +43,9 @@ Ltac red_obj_rule :=
       subst; clear H0 H2
     end.
 
-Ltac good_locking_rule_get rule :=
+Ltac good_rqrs_rule_get rule :=
   match goal with
-  | [H: GoodLockingSys _ ?sys,
+  | [H: GoodRqRsSys _ ?sys,
      Hobj: In ?obj (sys_objs ?sys),
      Hrule: In rule (obj_rules ?obj) |- _] =>
     let Hg := fresh "H" in
@@ -56,72 +56,56 @@ Ltac good_locking_rule_get rule :=
     specialize (Hg _ Hrule)
   end.
 
-Section RqUpInv.
+Ltac good_rqrs_rule_cases rule :=
+  match goal with
+  | [H: GoodRqRsRule _ _ rule |- _] =>
+    destruct H as [|[|[|[|]]]]
+  end.
+
+Section MessageInv.
   Context {oifc: OStateIfc}.
-  Variables (dtr: DTree)
+  Variables (gtr: DTree)
             (sys: System oifc).
 
-  Hypothesis (Hrrs: RqRsSys dtr sys).
-  
-  Lemma rqUp_reducible:
-    forall oidx1 ridx1 rins1 routs1 rule1 obj1
-           (Hobj1: In obj1 sys.(sys_objs)) (Hoidx1: obj1.(obj_idx) = oidx1)
-           (Hrule1: In rule1 obj1.(obj_rules))
-           (Hridx1: rule1.(rule_idx) = ridx1)
-           oidx2 ridx2 rins2 routs2 rule2 obj2
-           (Hobj2: In obj2 sys.(sys_objs)) (Hoidx2: obj2.(obj_idx) = oidx2)
-           (Hrule2: In rule2 obj2.(obj_rules))
-           (Hridx2: rule2.(rule_idx) = ridx2),
-      RqFromDownRule dtr oidx1 rule1 ->
-      RqToUpRule dtr oidx1 rule1 ->
-      DisjList routs1 rins2 ->
-      Reducible sys [RlblInt oidx2 ridx2 rins2 routs2;
-                       RlblInt oidx1 ridx1 rins1 routs1]
-                [RlblInt oidx1 ridx1 rins1 routs1;
-                   RlblInt oidx2 ridx2 rins2 routs2].
+  Hypothesis (Hitr: GoodRqRsSys gtr sys).
+
+  Definition RqUpMsgs (oidx: IdxT) (msgs: list (Id Msg)): Prop :=
+    exists rqUp, msgs = [rqUp] /\
+                 msg_type (valOf rqUp) = MRq /\
+                 In (idOf rqUp) (rqEdgesUpTo gtr oidx).
+
+  Definition RqDownMsgs (oidx: IdxT) (msgs: list (Id Msg)): Prop :=
+    exists rqDown, msgs = [rqDown] /\
+                   msg_type (valOf rqDown) = MRq /\
+                   edgeDownTo gtr oidx = Some (idOf rqDown).
+
+  Definition RsUpMsgs (oidx: IdxT) (msgs: list (Id Msg)): Prop :=
+    Forall (fun msg => msg_type (valOf msg) = MRs) msgs /\
+    SubList (idsOf msgs) (rsEdgesUpTo gtr oidx).
+
+  Definition RsDownMsgs (oidx: IdxT) (msgs: list (Id Msg)): Prop :=
+    exists rsDown, msgs = [rsDown] /\
+                   msg_type (valOf rsDown) = MRs /\
+                   edgeDownTo gtr oidx = Some (idOf rsDown).
+
+  Lemma messages_in_cases:
+    forall s1 oidx ridx rins routs s2,
+      step_m sys s1 (RlblInt oidx ridx rins routs) s2 ->
+      RqUpMsgs oidx rins \/
+      RqDownMsgs oidx rins \/
+      RsUpMsgs oidx rins \/
+      RsDownMsgs oidx rins.
   Proof.
     intros.
-    destruct Hrrs as [? [? ?]].
-    unfold Reducible; intros.
+    inv H.
+    good_rqrs_rule_get rule.
+    good_rqrs_rule_cases rule.
 
-    apply internal_commutes; auto.
-        
-    - inv_steps; inv_step.
-      red_obj_rule.
-      good_locking_rule_get rule2.
-
-      red.
-      destruct (eq_nat_dec (obj_idx obj) (obj_idx obj0));
-        [right|left; assumption].
-      red_obj_rule.
-      split; [reflexivity|]; intros.
-      red_obj_rule.
-
-      clear -H0 H H5.
-      red in H5; dest.
-      red; intros.
-      split.
+    - left.
 
       Ltac disc_rule_conds :=
         repeat
           (match goal with
-           | [H: RqFromDownRule _ _ _ |- _] =>
-             let rqFrom := fresh "rqFrom" in destruct H as [rqFrom ?]; dest
-           | [H: RqToUpRule _ _ _ |- _] =>
-             let rqTo := fresh "rqTo" in destruct H as [rqTo ?]; dest
-
-           | [H: MsgsFrom _ _ _ _ |- _] => red in H
-           | [H: MsgsTo _ _ |- _] => red in H
-           | [H: RqAccepting _ _ _ |- _] => red in H
-           | [H: RqReleasing _ |- _] => red in H
-           (* | [H: UpLockFree _ _ _ |- _] => red in H *)
-           (* | [H: UpLocking _ |- _] => red in H *)
-           (* | [H: UpLockedORq _ _ |- _] => red in H *)
-           (* | [H: DownLockFree _ _ _ |- _] => red in H *)
-           (* | [H: DownLocking _ |- _] => red in H *)
-           (* | [H: DownLockedORq _ _ |- _] => red in H *)
-           | [H: StateUnchanged _ |- _] => red in H
-                                                    
            | [H1: rule_precond ?rule ->oprec _, H2: rule_precond ?rule _ _ _ |- _] =>
              specialize (H1 _ _ _ H2)
            | [H: (_ /\oprec _) _ _ _ |- _] => destruct H
@@ -129,18 +113,177 @@ Section RqUpInv.
              specialize (H2 ost orq ins); rewrite H1 in H2; simpl in H2
            end; simpl in *; subst).
 
-      + disc_rule_conds.
-        eapply H3; [eassumption|].
-        eapply UpLockFree_UpLocking_SubLock; eauto.
-
-      + (* Conjecture: it's just about postconditions, thus provable by
-         * the case analysis on [GoodLockingRelease] *)
-        admit.
-
-    - admit.
-    - admit.
-
   Admitted.
+    
+End MessageInv.
+
+(** NOTE: With [LockInv] below we may need some invariants 
+ * for [Atomic] histories, such as: if [Atomic hst] and [st1 -(hst)-> st2]
+ * then [hst.eouts ⊆ st2.msgs].
+ *)
+
+(* Want: between two continuous histories H1 and H2, after H1, related locks are
+ * never released until H2; it can be proven by [LockInv] below and
+ * [atomic_messages_spec_in] in SerialFacts.v.
+ *)
+Section LockInv.
+  Context {oifc: OStateIfc}.
+  Variables (dtr: DTree)
+            (sys: System oifc).
+
+  Hypothesis (Hrr: GoodRqRsSys dtr sys).
+
+  Section OnMState.
+    Variables (orqs: ORqs Msg)
+              (msgs: MessagePool Msg).
+
+    Definition OUpLocked (oidx: IdxT) :=
+      orqs@[oidx] >>=[False] (fun orq => UpLockedORq orq).
+
+    Definition ODownLocked (oidx: IdxT) :=
+      orqs@[oidx] >>=[False] (fun orq => DownLockedORq orq).
+
+    Definition OUpLockFree (oidx: IdxT) :=
+      orqs@[oidx] >>=[True] (fun orq => UpLockFreeORq orq).
+
+    Definition ODownLockFree (oidx: IdxT) :=
+      orqs@[oidx] >>=[True] (fun orq => DownLockFreeORq orq).
+
+    Definition rqsQ (midx: IdxT) :=
+      filter (fun msg => msg.(msg_type) ==n MRq) (findQ midx msgs).
+
+    Definition rssQ (midx: IdxT) :=
+      filter (fun msg => msg.(msg_type) ==n MRs) (findQ midx msgs).
+
+    Definition UpLockFreeInv (oidx: IdxT) :=
+      (rqEdgeUpFrom dtr oidx) >>=[True] (fun rqUp => findQ rqUp msgs = nil) /\
+      (edgeDownTo dtr oidx) >>=[True] (fun down => rssQ down = nil) /\
+      (parentOf dtr oidx) >>=[True] (fun pidx => OUpLockFree pidx).
+    
+    Definition UpLockedInv (oidx: IdxT) :=
+      exists rqUp down pidx,
+        rqEdgeUpFrom dtr oidx = Some rqUp /\
+        edgeDownTo dtr oidx = Some down /\
+        parentOf dtr oidx = Some pidx /\
+        xor3 (findQ rqUp msgs <> nil)
+             (rssQ down <> nil)
+             (OUpLocked pidx).
+
+    Definition DownLockFreeInv (oidx: IdxT) :=
+      forall cidx,
+        parentOf dtr cidx = Some oidx ->
+        ((edgeDownTo dtr cidx) >>=[True] (fun down => rqsQ down = nil) /\
+         (rsEdgeUpFrom dtr cidx) >>=[True] (fun rsUp => findQ rsUp msgs = nil)).
+    
+    Definition DownLockedInv (oidx: IdxT) (rqi: RqInfo Msg) :=
+      Forall (fun rsUp =>
+                exists down cidx,
+                  edgeDownTo dtr cidx = Some down /\
+                  rsEdgeUpFrom dtr cidx = Some rsUp /\
+                  parentOf dtr cidx = Some oidx /\
+                  xor (rqsQ down <> nil) (findQ rsUp msgs <> nil))
+             rqi.(rqi_minds_rss).
+
+    Definition UpLockInvORq (oidx: IdxT) (orq: ORq Msg) :=
+      match orq@[upRq] with
+      | Some _ => UpLockedInv oidx
+      | None => UpLockFreeInv oidx
+      end.
+
+    Definition DownLockInvORq (oidx: IdxT) (orq: ORq Msg) :=
+      match orq@[downRq] with
+      | Some downRqi => DownLockedInv oidx downRqi
+      | None => DownLockFreeInv oidx
+      end.
+
+    Definition LockInvMO :=
+      forall oidx,
+        In oidx (map (@obj_idx _) sys.(sys_objs)) ->
+        let orq := orqs@[oidx] >>=[[]] (fun orq => orq) in
+        UpLockInvORq oidx orq /\ DownLockInvORq oidx orq.
+
+  End OnMState.
+  
+  Definition LockInv (st: MState oifc) :=
+    LockInvMO st.(bst_orqs) st.(bst_msgs).
+
+  Lemma lockInv_init:
+    sys.(sys_orqs_inits) = [] ->
+    InvInit sys LockInv.
+  Proof.
+    intros; do 3 red; cbn.
+    intros; cbn; rewrite H; cbn.
+    split.
+    - red; cbn; repeat split.
+      + destruct (rqEdgeUpFrom dtr oidx); simpl; auto.
+      + destruct (edgeDownTo dtr oidx); simpl; auto.
+      + destruct (parentOf dtr oidx); simpl; auto.
+    - red; cbn; repeat split.
+      + destruct (edgeDownTo dtr cidx); simpl; auto.
+      + destruct (rsEdgeUpFrom dtr cidx); simpl; auto.
+  Qed.
+
+  Lemma lockInv_step_ext_in:
+    forall oss orqs msgs eins,
+      LockInv {| bst_oss := oss; bst_orqs := orqs; bst_msgs := msgs |} ->
+      eins <> nil ->
+      ValidMsgsExtIn sys eins ->
+      LockInv {| bst_oss := oss;
+                 bst_orqs := orqs;
+                 bst_msgs := enqMsgs eins msgs |}.
+  Proof.
+  Admitted.
+
+  Lemma lockInv_step_ext_out:
+    forall oss orqs msgs eouts,
+      LockInv {| bst_oss := oss; bst_orqs := orqs; bst_msgs := msgs |} ->
+      eouts <> nil ->
+      Forall (FirstMPI msgs) eouts ->
+      ValidMsgsExtOut sys eouts ->
+      LockInv {| bst_oss := oss;
+                 bst_orqs := orqs;
+                 bst_msgs := deqMsgs (idsOf eouts) msgs |}.
+  Proof.
+  Admitted.
+  
+  Lemma lockInv_step:
+    InvStep sys step_m LockInv.
+  Proof.
+    red; intros.
+    
+    inv H1; auto.
+    - apply lockInv_step_ext_in; auto.
+    - apply lockInv_step_ext_out; auto.
+    - 
+  Admitted.
+
+End LockInv.
+
+Section RqUpInv.
+  Context {oifc: OStateIfc}.
+  Variables (dtr: DTree)
+            (sys: System oifc).
+
+  Hypothesis (Hrrs: GoodRqRsSys dtr sys)
+             (Hrud: RqUpRsUpOkSys dtr sys).
+  
+  (* Lemma rqUp_reducible: *)
+  (*   forall oidx1 ridx1 rins1 routs1 rule1 obj1 *)
+  (*          (Hobj1: In obj1 sys.(sys_objs)) (Hoidx1: obj1.(obj_idx) = oidx1) *)
+  (*          (Hrule1: In rule1 obj1.(obj_rules)) *)
+  (*          (Hridx1: rule1.(rule_idx) = ridx1) *)
+  (*          oidx2 ridx2 rins2 routs2 rule2 obj2 *)
+  (*          (Hobj2: In obj2 sys.(sys_objs)) (Hoidx2: obj2.(obj_idx) = oidx2) *)
+  (*          (Hrule2: In rule2 obj2.(obj_rules)) *)
+  (*          (Hridx2: rule2.(rule_idx) = ridx2), *)
+  (*     RqToUpRule dtr oidx1 rule1 -> *)
+  (*     DisjList routs1 rins2 -> *)
+  (*     Reducible sys [RlblInt oidx2 ridx2 rins2 routs2; *)
+  (*                      RlblInt oidx1 ridx1 rins1 routs1] *)
+  (*               [RlblInt oidx1 ridx1 rins1 routs1; *)
+  (*                  RlblInt oidx2 ridx2 rins2 routs2]. *)
+  (* Proof. *)
+  (* Admitted. *)
 
 End RqUpInv.
 
@@ -196,81 +339,12 @@ Definition trsTypeOf (gtr: DTree) (idm: Id Msg):
         | CDown => if eq_nat_dec (msg_type (snd idm)) MRq then RqDown else RsDown
         end)).
 
-Section MessageInv.
-  Context {oifc: OStateIfc}.
-  Variables (gtr: DTree)
-            (sys: System oifc).
-
-  Hypothesis (Hitr: GoodIterationSys gtr sys).
-
-  Definition RqUpMsgs (oidx: IdxT) (msgs: list (Id Msg)): Prop :=
-    exists rqUp, msgs = [rqUp] /\
-                 msg_type (valOf rqUp) = MRq /\
-                 In (idOf rqUp) (rqEdgesUpTo gtr oidx).
-
-  Definition RqDownMsgs (oidx: IdxT) (msgs: list (Id Msg)): Prop :=
-    exists rqDown, msgs = [rqDown] /\
-                   msg_type (valOf rqDown) = MRq /\
-                   edgeDownTo gtr oidx = Some (idOf rqDown).
-
-  Definition RsUpMsgs (oidx: IdxT) (msgs: list (Id Msg)): Prop :=
-    Forall (fun msg => msg_type (valOf msg) = MRs) msgs /\
-    SubList (idsOf msgs) (rsEdgesUpTo gtr oidx).
-
-  Definition RsDownMsgs (oidx: IdxT) (msgs: list (Id Msg)): Prop :=
-    exists rsDown, msgs = [rsDown] /\
-                   msg_type (valOf rsDown) = MRs /\
-                   edgeDownTo gtr oidx = Some (idOf rsDown).
-
-  Lemma messages_in_cases:
-    forall s1 oidx ridx rins routs s2,
-      step_m sys s1 (RlblInt oidx ridx rins routs) s2 ->
-      RqUpMsgs oidx rins \/
-      RqDownMsgs oidx rins \/
-      RsUpMsgs oidx rins \/
-      RsDownMsgs oidx rins.
-  Proof.
-    intros.
-    inv H.
-
-    pose proof Hitr.
-    red in H; rewrite Forall_forall in H.
-    specialize (H _ H4).
-    red in H; rewrite Forall_forall in H.
-    specialize (H _ H5).
-    red in H.
-    destruct H as [|[|[|[|]]]].
-
-    - left.
-      admit.
-    - right; left.
-
-      red in H.
-      destruct H as [rqFrom [rsTo ?]]; dest.
-      specialize (H1 _ _ _ H11).
-      destruct H1.
-      red in H1.
-      red in H6.
-
-      destruct rins; try discriminate.
-      destruct rins; try discriminate.
-      destruct i as [i v]; simpl in *.
-      inv H1; inv H6; clear H17; simpl in *.
-
-      exists (rqFrom, v); repeat split; auto.
-    - admit.
-    - admit.
-    - admit.
-  Admitted.
-    
-End MessageInv.
-
 Section AtomicInv.
   Context {oifc: OStateIfc}.
   Variables (gtr: DTree)
             (sys: System oifc).
 
-  Hypothesis (Hitr: GoodIterationSys gtr sys).
+  Hypothesis (Hitr: GoodRqRsSys gtr sys).
 
   Definition subtreeInds (sroot: option IdxT): list IdxT :=
     sroot >>=[nil] (fun sroot => dg_vs (topoOfT (subtree gtr sroot))).
@@ -305,8 +379,6 @@ Section AtomicInv.
 
   Definition AtomicInv (inits eouts: list (Id Msg)) (hst: MHistory) :=
     NoDup (rssOf hst) /\
-    SubList (rssOf hst) (rsDownCovers inits) /\
-    DisjList (rssOf hst) (rsUpCovers inits) /\
     SubList (rssOf hst) (rsUpCovers eouts) /\
     DisjList (rssOf hst) (rsDownCovers eouts).
 
@@ -317,145 +389,9 @@ Section AtomicInv.
         steps step_m sys s1 hst s2 ->
         AtomicInv inits eouts hst.
   Proof.
-    induction 1; simpl; intros; subst.
-    
-    - inv H; inv H3; inv H5.
-
-      pose proof Hitr.
-      red in H; rewrite Forall_forall in H.
-      specialize (H _ H3).
-      red in H; rewrite Forall_forall in H.
-      specialize (H _ H4).
-      red in H.
-
-      (* destruct H as [ *)
-
-      
-
   Admitted.
   
 End AtomicInv.
-
-(* Want: between two continuous histories H1 and H2, after H1, related locks are
- * never released until H2; it can be proven by [LockInv] below and
- * [atomic_messages_spec_in] in SerialFacts.v.
- *)
-Section LockInv.
-  Context {oifc: OStateIfc}.
-  Variables (gtr: DTree)
-            (sys: System oifc).
-
-  Hypothesis (Hrr: GoodLockingSys gtr sys).
-
-  Section OnMState.
-    Variables (orqs: ORqs Msg)
-              (msgs: MessagePool Msg).
-
-    Definition OLocked (oidx: IdxT) :=
-      orqs@[oidx] >>=[False]
-        (fun orq => orq@[downRq] <> None).
-
-    Definition DownLockFreeInv (oidx: IdxT) :=
-      let str := subtree gtr oidx in
-      ForallQ (fun midx q =>
-                 if midx ?<n (rsUpEdges str)
-                 then q = nil
-                 else if midx ?<n (downEdges str)
-                      then filter (fun msg => msg.(msg_type) ==n MRq) q = nil
-                      else True) msgs.
-
-    Definition DownLockedInv (oidx: IdxT) (rqi: RqInfo Msg) :=
-      let str := subtree gtr oidx in
-      let ctrs := childrenOf str in
-      Forall (fun child =>
-                match child with
-                | Leaf => True
-                | Node croot _ =>
-                  (rsEdgeUpFrom gtr croot)
-                    >>=[True]
-                    (fun rsUp =>
-                       if rsUp ?<n rqi.(rqi_minds_rss)
-                       then (edgeDownTo gtr croot)
-                              >>=[True]
-                              (fun down =>
-                                 xor3 (length (findQ rsUp msgs) = 1)
-                                      (length (filter (fun msg => msg.(msg_type) ==n MRq)
-                                                      (findQ down msgs)) = 1)
-                                      (OLocked croot))
-                       else DownLockFreeInv croot)
-                end) ctrs.
-
-    Definition LockInvORq (oidx: IdxT) (orq: ORq Msg) :=
-      match orq@[downRq] with
-      | Some downRqi => DownLockedInv oidx downRqi
-      | None => DownLockFreeInv oidx
-      end.
-
-    Definition LockInvMO :=
-      forall oidx,
-        In oidx (map (@obj_idx _) sys.(sys_objs)) ->
-        LockInvORq oidx (orqs@[oidx] >>=[[]] (fun orq => orq)).
-
-  End OnMState.
-  
-  Definition LockInv (st: MState oifc) :=
-    LockInvMO st.(bst_orqs) st.(bst_msgs).
-
-  Lemma lockInv_init:
-    sys.(sys_orqs_inits) = [] ->
-    InvInit sys LockInv.
-  Proof.
-    intros; do 3 red; cbn.
-    intros; cbn; rewrite H; cbn.
-    do 2 red; cbn; intros.
-    find_if_inside; auto.
-    find_if_inside; auto.
-  Qed.
-
-  Lemma lockInv_step_ext_in:
-    forall oss orqs msgs eins,
-      LockInv {| bst_oss := oss; bst_orqs := orqs; bst_msgs := msgs |} ->
-      eins <> nil ->
-      ValidMsgsExtIn sys eins ->
-      LockInv {| bst_oss := oss;
-                 bst_orqs := orqs;
-                 bst_msgs := enqMsgs eins msgs |}.
-  Proof.
-    unfold LockInv, LockInvMO; cbn; intros.
-    specialize (H oidx H2).
-    unfold LockInvORq in *.
-    remember (orqs@[oidx]) as orq; destruct orq as [orq|]; cbn in *.
-    - remember (orq@[0]) as aorq; destruct aorq as [aorq|]; cbn in *.
-      + admit.
-      + admit.
-    - admit.
-    
-  Admitted.
-
-  Lemma lockInv_step_ext_out:
-    forall oss orqs msgs eouts,
-      LockInv {| bst_oss := oss; bst_orqs := orqs; bst_msgs := msgs |} ->
-      eouts <> nil ->
-      Forall (FirstMPI msgs) eouts ->
-      ValidMsgsExtOut sys eouts ->
-      LockInv {| bst_oss := oss;
-                 bst_orqs := orqs;
-                 bst_msgs := deqMsgs (idsOf eouts) msgs |}.
-  Proof.
-  Admitted.
-  
-  Lemma lockInv_step:
-    InvStep sys step_m LockInv.
-  Proof.
-    red; intros.
-    
-    inv H1; auto.
-    - apply lockInv_step_ext_in; auto.
-    - apply lockInv_step_ext_out; auto.
-    - 
-  Admitted.
-
-End LockInv.
 
 Close Scope list.
 Close Scope fmap.
